thys/Formula.thy
@@ -659,7 +659,7 @@ and safe_regex :: "modality \<Rightarrow> safety \<Rightarrow> 'a regex \<Righta
 | "safe_formula (Ands l) = (let (pos, neg) = partition safe_formula l in pos \<noteq> [] \<and>
     list_all safe_formula (map remove_neg neg) \<and> \<Union>(set (map fv neg)) \<subseteq> \<Union>(set (map fv pos)))"
 | "safe_formula (Exists \<phi>) = (safe_formula \<phi>)"
-| "safe_formula (Agg y \<omega> b f \<phi>) = (safe_formula \<phi> \<and> y + b \<notin> fv \<phi>)"
+| "safe_formula (Agg y \<omega> b f \<phi>) = (safe_formula \<phi> \<and> y + b \<notin> fv \<phi> \<and> {..<b} \<subseteq> fv \<phi>)"
 | "safe_formula (Prev I \<phi>) = (safe_formula \<phi>)"
 | "safe_formula (Next I \<phi>) = (safe_formula \<phi>)"
 | "safe_formula (Since \<phi> I \<psi>) = (fv \<phi> \<subseteq> fv \<psi> \<and>
@@ -774,7 +774,7 @@ lemma safe_formula_regex_induct[consumes 2]:
               fv \<phi> = {} \<Longrightarrow> safe_formula \<phi> \<Longrightarrow> P \<phi> \<Longrightarrow> P (Neg \<phi>)"
     and "\<And>\<phi> \<psi>. fv \<psi> = fv \<phi> \<Longrightarrow> P \<phi> \<Longrightarrow> P \<psi> \<Longrightarrow> P (Or \<phi> \<psi>)"
     and "\<And>\<phi>. P \<phi> \<Longrightarrow> P (Exists \<phi>)"
-    and "\<And>y \<omega> b f \<phi>. y + b \<notin> fv \<phi> \<Longrightarrow> P \<phi> \<Longrightarrow> P (Agg y \<omega> b f \<phi>)"
+    and "\<And>y \<omega> b f \<phi>. y + b \<notin> fv \<phi> \<Longrightarrow> {..<b} \<subseteq> fv \<phi> \<Longrightarrow> P \<phi> \<Longrightarrow> P (Agg y \<omega> b f \<phi>)"
     and "\<And>I \<phi>. P \<phi> \<Longrightarrow> P (Prev I \<phi>)"
     and "\<And>I \<phi>. P \<phi> \<Longrightarrow> P (Next I \<phi>)"
     and "\<And>\<phi> I \<psi>. fv \<phi> \<subseteq> fv \<psi> \<Longrightarrow> safe_formula \<phi> \<Longrightarrow> P \<phi> \<Longrightarrow> P \<psi> \<Longrightarrow> P (Since \<phi> I \<psi>)"
@@ -849,7 +849,7 @@ lemma safe_formula_induct[consumes 1]:
               fv \<phi> = {} \<Longrightarrow> safe_formula \<phi> \<Longrightarrow> P \<phi> \<Longrightarrow> P (Neg \<phi>)"
     and "\<And>\<phi> \<psi>. fv \<psi> = fv \<phi> \<Longrightarrow> P \<phi> \<Longrightarrow> P \<psi> \<Longrightarrow> P (Or \<phi> \<psi>)"
     and "\<And>\<phi>. P \<phi> \<Longrightarrow> P (Exists \<phi>)"
-    and "\<And>y \<omega> b f \<phi>. y + b \<notin> fv \<phi> \<Longrightarrow> P \<phi> \<Longrightarrow> P (Agg y \<omega> b f \<phi>)"
+    and "\<And>y \<omega> b f \<phi>. y + b \<notin> fv \<phi> \<Longrightarrow> {..<b} \<subseteq> fv \<phi> \<Longrightarrow> P \<phi> \<Longrightarrow> P (Agg y \<omega> b f \<phi>)"
     and "\<And>I \<phi>. P \<phi> \<Longrightarrow> P (Prev I \<phi>)"
     and "\<And>I \<phi>. P \<phi> \<Longrightarrow> P (Next I \<phi>)"
     and "\<And>\<phi> I \<psi>. fv \<phi> \<subseteq> fv \<psi> \<Longrightarrow> safe_formula \<phi> \<Longrightarrow> P \<phi> \<Longrightarrow> P \<psi> \<Longrightarrow> P (Since \<phi> I \<psi>)"
